src/ReactorModel/Determinism/State.lean
@@ -1,0 +1,132 @@
+import ReactorModel.Determinism.Dependency
+
+open ReactorType
+
+namespace Execution
+namespace State
+
+theorem exec_equiv {s : State} {rcn : s.rtr.Valid .rcn} : s.rtr ≈ (s.exec rcn).rtr := 
+  Equivalent.symm $ Reactor.apply'_equiv _ _
+
+set_option pp.proofs.withType false
+theorem exec_indep_input_state_eq  {s : State} {rcn₁ rcn₂ : s.rtr.Valid .rcn} (hn : rcn₁ ≠ rcn₂) 
+    (hi : rcn₁ ≮[s.rtr] rcn₂) : input.state (s.exec rcn₁) rcn₂.equiv = input.state s rcn₂ := by 
+  simp [input.state]
+  set rcn₂' := rcn₂.equiv (rtr₂ := (s.exec rcn₁).rtr)
+  have h₁ := rcn₂.con?_id_eq_con
+  have h₂ := rcn₂'.con?_id_eq_con
+  set con₁ := rcn₂.con
+  set con₂ := rcn₂'.con
+  cases hi.ne_con_or_pure hn <;> try cases ‹_ ∨ _›  
+  case _ hc =>
+    sorry
+  case _ hc =>
+    sorry -- use Pure.output
+  case _ hc =>
+    simp [exec] at h₂ -- use Pure.input
+    sorry
+
+theorem exec_indep_input_ports_eq {s : State} {rcn₁ rcn₂ : s.rtr.Valid .rcn} (hn : rcn₁ ≠ rcn₂)
+    (hi : rcn₁ ≮[s.rtr] rcn₂) : input.ports (s.exec rcn₁) rcn₂.equiv = input.ports s rcn₂ := by 
+  sorry
+  
+theorem exec_indep_input_acts_eq {s : State} {rcn₁ rcn₂ : s.rtr.Valid .rcn} (hn : rcn₁ ≠ rcn₂)
+    (hi : rcn₁ ≮[s.rtr] rcn₂) : input.acts (s.exec rcn₁) rcn₂.equiv = input.acts s rcn₂ := by 
+  sorry
+
+theorem exec_indep_input_eq (s : State) {rcn₁ rcn₂ : s.rtr.Valid .rcn} (hn : rcn₁ ≠ rcn₂)
+    (hi : rcn₁ ≮[s.rtr] rcn₂) : (s.exec rcn₁).input rcn₂.equiv = s.input rcn₂ := by 
+  simp [input]
+  refine ⟨?ports, ?acts, ?state, rfl⟩
+  case state => exact exec_indep_input_state_eq hn hi
+  case ports => exact exec_indep_input_ports_eq hn hi
+  case acts  => exact exec_indep_input_acts_eq hn hi
+    
+    /-
+theorem InstStep.indep_rcns_indep_output :
+  (e : s ⇓ᵢ s') → (rcn' <[s.rtr]> e.rcn) → (rcn' ≠ e.rcn) → s.output rcn' = s'.rcnOutput rcn' := by
+  intro h hi hrne
+  have hp := h.exec.preserves_rcns
+  cases ho : s.rtr[.rcn][rcn'] <;> cases ho' : s'.rtr[.rcn][rcn']
+  case none.none => simp [State.rcnOutput, ho, ho']
+  case' none.some, some.none => simp [hp, ho'] at ho
+  case some.some => 
+    have ⟨⟨p, a, x, t⟩, hj⟩ := State.rcnInput_iff_obj?.mpr ⟨_, ho⟩
+    have ⟨⟨p', a', x', t'⟩, hj'⟩ := State.rcnInput_iff_obj?.mpr ⟨_, ho'⟩
+    have H1 : p = p' := by 
+      simp [s.rcnInput_ports_def hj ho, s'.rcnInput_ports_def hj' ho']
+      rw [←hp] at ho'
+      have he := Option.some_inj.mp $ ho.symm.trans ho'
+      simp [he]
+      sorry
+    sorry
+      
+      refine congr_arg₂ _ ?_ rfl
+      apply Finmap.restrict_ext
+      intro p hp
+      have ⟨_, hr⟩ := Reactor.contains_iff_obj?.mp h.rtr_contains_rcn
+      have hd := hi.symm.nonoverlapping_deps hr ho'
+      simp [Finset.eq_empty_iff_forall_not_mem, Finset.mem_inter] at hd
+      have hd := mt (hd p) $ not_not.mpr hp
+      simp [Reactor.obj?'_eq_obj?, h.preserves_nondep_ports hr hd]
+    have H2 : a = a' := by
+      simp [s.rcnInput_actions_def hj ho, s'.rcnInput_actions_def hj' ho']
+      rw [←hp] at ho'
+      have he := Option.some_inj.mp $ ho.symm.trans ho'
+      simp [he]
+      apply Finmap.restrict_ext
+      intro a ha
+      simp [h.preserves_tag]
+      apply Finmap.filterMap_congr
+      have ⟨_, hr⟩ := Reactor.contains_iff_obj?.mp h.rtr_contains_rcn
+      have hd := hi.symm.nonoverlapping_deps hr ho'
+      simp [Finset.eq_empty_iff_forall_not_mem, Finset.mem_inter] at hd
+      have hd := mt (hd a) $ not_not.mpr ha
+      simp [Reactor.obj?'_eq_obj?, h.preserves_nondep_actions hr hd]
+    have H3 : t = t' := by 
+      simp [s.rcnInput_time_def hj, s'.rcnInput_time_def hj', h.exec.preserves_tag]
+    simp [H1, H2, H3] at hj
+    have ⟨r, hr⟩ := Reactor.contains_iff_obj?.mp h.rtr_contains_rcn
+    have ⟨_, hc, _⟩ := Reactor.obj?_to_con?_and_cpt? ho
+    have ⟨_, hr', _⟩ := Reactor.obj?_to_con?_and_cpt? hr
+    cases hi.ne_rtr_or_pure hrne ho hr hc hr'
+    case inl he => 
+      have ⟨_, hc', _⟩ := Reactor.obj?_to_con?_and_cpt? ho'
+      have hs := State.rcnInput_state_def hj hc
+      have hs' := State.rcnInput_state_def hj' hc'
+      have hq := h.exec.equiv
+      have hh := hq.con?_id_eq hc hc'
+      have hc := Reactor.con?_to_rtr_obj? hc
+      have hc' := Reactor.con?_to_rtr_obj? hc'
+      rw [←hh] at hc'
+      rw [h.preserves_external_state hr' hc hc' he.symm] at hs
+      rw [hs.trans hs'.symm] at hj
+      exact State.rcnOutput_congr (hj.trans hj'.symm) hp
+    case inr hc =>
+      cases hc
+      case inl hp' => 
+        rw [ho'.symm.trans (h.exec.preserves_rcns ▸ ho)] at ho'
+        exact State.rcnOutput_pure_congr hj hj' ho ho' hp'
+      case inr hp' => 
+        have ⟨_, hco, _⟩ := Reactor.obj?_to_con?_and_cpt? ho
+        have ⟨_, hco', _⟩ := Reactor.obj?_to_con?_and_cpt? ho'
+        have hs := State.rcnInput_state_def hj hco
+        have hs' := State.rcnInput_state_def hj' hco'
+        suffices h : x = x' by 
+          rw [h] at hj
+          exact State.rcnOutput_congr (hj.trans hj'.symm) hp
+        rw [hs, hs']
+        have he := h.exec.equiv
+        exact (he.con?_obj_equiv hco hco').obj?_ext (cpt := .stv) (by
+          intro j _
+          have h := h.pure_preserves_state (j := j) hr hp'
+          have hh := he.con?_id_eq hco hco'
+          have hco := Reactor.con?_to_rtr_obj? hco
+          have hco' := Reactor.con?_to_rtr_obj? hco'
+          rw [←hh] at hco'
+          exact he.eq_obj?_nest h hco hco' 
+        )
+    -/
+
+namespace State
+namespace Execution
